src/Language/Marlowe/Examples/Rent.hs
@@ -4,7 +4,7 @@ module Language.Marlowe.Examples.Rent where
 import Language.Marlowe
 
 utility :: Contract
-utility = mkDeposit $ payMonth 1 $ payMonth 2 $ payMonth 3 $ Refund
+utility = mkDeposit $ payMonth 1 $ payMonth 2 $ payMonth 3 $ Close
 
 tenant, landlord :: Party
 tenant = "tenant"
@@ -27,12 +27,12 @@ daysInAMonth = 30
 mkDeposit c = When [Case (Deposit depositAcc tenant (Constant depositAmt))
                          c]
                    depositTimeout
-                   Refund
+                   Close
 
 payMonth m c = When [Case (Deposit monthlyAcc tenant (Constant monthlyFee))
                           (payAll monthlyAcc (Party landlord) c)]
                     (depositTimeout + m * daysInAMonth)
-                    (payAll depositAcc (Party landlord) Refund)
+                    (payAll depositAcc (Party landlord) Close)
 
 -- Pay all money into an account to a payee
 payAll :: AccountId -> Payee -> Contract -> Contract
